Finish the generalization of the FirstChar splitter

src/Parsers/Splitters/OnlyOneNonterminal.v
@@ -21,13 +21,16 @@ Local Open Scope string_scope.
 Local Open Scope string_like_scope.
 
 Local Coercion is_true : bool >-> Sortclass.
+
+Create HintDb equality_t_db discriminated.
+Create HintDb equality_t_end_db discriminated.
+
 Section StringT.
   Context {CharType} {String : string_like CharType} (split_stateT : String -> Type).
 
   Let String' : Type := String.
   Let StringT := (StringWithSplitState String split_stateT).
-About eq_rect.
-About RightId.
+
   Context (empty_state : split_stateT (Empty _))
           (split_state_at : forall n s,
                               split_stateT s
@@ -66,12 +69,20 @@ About RightId.
                  | generalize a; generalize b; intros; progress subst ]
     end.
 
+  Hint Rewrite RightId LeftId @substring_correct3' Bool.orb_true_r : equality_t_db.
+  Hint Rewrite Singleton_Length : equality_t_end_db.
+  Hint Rewrite <- Length_correct : equality_t_end_db.
+
   Local Ltac t_equality :=
     repeat match goal with
              | _ => intro
              | _ => reflexivity
-             | [ H : is_true false |- _ ] => hnf in H; clear -H; exfalso; abstract discriminate
-             | [ H : false = true |- _ ] => hnf in H; clear -H; exfalso; abstract discriminate
+             | [ H : is_true false |- _ ] => hnf in H; exfalso; clear -H; abstract discriminate
+             | [ H : false = true |- _ ] => exfalso; clear -H; abstract discriminate
+             | [ H : ?x = true, H' : ?x = false |- _ ]
+               => symmetry in H';
+                 assert (false = true) by (etransitivity; [ exact H' | exact H ]);
+                 clear H H'
              | _ => progress simpl in *
              | _ => progress subst
              | _ => progress destruct_head sigT
@@ -79,14 +90,12 @@ About RightId.
              | _ => progress destruct_head and
              | _ => progress destruct_head @StringWithSplitState
              | [ |- _ = _ :> (_ * _)%type ] => apply f_equal2
-             (*| [ |- _ = _ :> StringT ] => apply StringT_eq*)
              | [ |- _ \/ False ] => left
-             | _ => rewrite RightId
-             | _ => rewrite LeftId
+             | _ => progress autorewrite with equality_t_db
              | [ H : context[string_dec ?str ?x] |- _ ] => atomic x; destruct (string_dec str x)
              | [ |- context[match ?s with _ => _ end] ] => atomic s; destruct s
              | [ H : context[match ?s with _ => _ end] |- _ ] => atomic s; destruct s
-             | _ => rewrite substring_correct3'
+             | [ |- context[match ?f ?x with true => _ | false => _ end] ] => atomic f; atomic x; case_eq (f x)
              | [ |- context[SplitAt ?n (?s1 ++ ?s2)] ]
                => replace n with (Length s1) by (rewrite Singleton_Length; trivial);
                  rewrite SplitAt_concat_correct
@@ -94,26 +103,27 @@ About RightId.
              | [ H : (_ || _ = false)%bool |- _ ] => apply Bool.orb_false_iff in H
              | [ H : (_ && _ = true)%bool |- _ ] => apply Bool.andb_true_iff in H
              | [ H : (_ && _ = false)%bool |- _ ] => apply Bool.andb_false_iff in H
-             | _ => rewrite Bool.orb_true_r
              | [ H : _ |- _ ] => rewrite Bool.orb_true_r in H
              | [ H : _ |- _ ] => rewrite H
              | _ => progress destruct_head or
-             | [ H : minimal_parse_of_item _ _ _ _ _ _ _ _ (Terminal _) |- _ ] => inversion H; clear H
-             | [ H : minimal_parse_of_item _ _ _ _ _ _ _ _ (NonTerminal _) |- _ ] => inversion H; clear H
-             | [ H : minimal_parse_of_production _ _ _ _ _ _ _ _ (_::_) |- _ ] => inversion H; clear H
-             | [ H : minimal_parse_of_production _ _ _ _ _ _ _ _ nil |- _ ] => inversion H; clear H
-             | _ => rewrite Singleton_Length
+             | [ H : minimal_parse_of_item _ _ _ (Terminal _) |- _ ] => inversion H; clear H
+             | [ H : minimal_parse_of_item _ _ _ (NonTerminal _) |- _ ] => inversion H; clear H
+             | [ H : minimal_parse_of_production _ _ _ (_::_) |- _ ] => inversion H; clear H
+             | [ H : minimal_parse_of_production _ _ _ nil |- _ ] => inversion H; clear H
+             | _ => progress autorewrite with equality_t_end_db
              | _ => progress unfold eq_rect
+             | [ |- In _ (@map nat _ _ _) ]
+               => apply in_map_iff; eexists; split; [ reflexivity | ]
              | [ |- context[match ?e with eq_refl => _ end] ] => destruct_matched_equality e
              | _ => solve [ eauto ]
            end.
 
-  Section first_char_splitter.
+  Section only_one_nt_splitter.
     Context (fallback_split
              : forall (it : item CharType)
                       (its : production CharType)
                       (str : StringT),
-                 list (StringT * StringT)).
+                 list nat).
 
     Fixpoint has_only_terminals (its : production CharType)
     : bool
@@ -123,7 +133,7 @@ About RightId.
            | (NonTerminal _)::_ => false
          end.
 
-    Definition first_char_split
+    Definition only_one_nt_split
                (it : item CharType)
                (its : production CharType)
                (str : StringT)
@@ -136,18 +146,18 @@ About RightId.
            | NonTerminal _, _
              => if has_only_terminals its
                 then [SplitAtT (Length str - List.length its) str]
-                else fallback_split it its str
+                else map (fun n => SplitAtT n str) (fallback_split it its str)
          end.
 
-    Lemma first_char_split_correct_seq {it its} {str : StringT}
+    Lemma only_one_nt_split_correct_seq {it its} {str : StringT}
           (f := fun strs : StringT * StringT => fst strs ++ snd strs =s str)
-          (fallback_split_correct_eq : List.Forall f (fallback_split it its str))
-    : List.Forall f (first_char_split it its str).
+    : List.Forall f (only_one_nt_split it its str).
     Proof.
-      unfold first_char_split; subst f.
+      unfold only_one_nt_split; subst f.
       repeat match goal with
                | _ => reflexivity
                | _ => assumption
+               | _ => intro
                | _ => progress simpl in *
                | [ |- context[match ?l with _ => _ end] ]
                  => atomic l; destruct l
@@ -156,54 +166,51 @@ About RightId.
                | _ => apply SplitAt_correct
                | [ |- List.Forall _ [] ] => constructor
                | [ |- List.Forall _ (_::_) ] => constructor
+               | [ |- List.Forall _ (map _ _) ] => apply Forall_map; unfold compose
+               | [ |- @List.Forall nat _ _ ] => apply Forall_forall
                | [ |- context[match ?l with _ => _ end] ]
                  => destruct l
              end.
     Qed.
 
     Context (G : grammar CharType).
-    Context (fallback_split_correct_eq
-             : forall it its (str : StringT),
-                 List.Forall
-                   (fun strs : StringT * StringT => fst strs ++ snd strs =s str)
-                   (fallback_split it its str)).
 
     Let data' : @parser_computational_types_dataT _ String
       := {| BaseTypes.predata := @rdp_list_predata _ G;
             BaseTypes.split_stateT str0 valid g := split_stateT |}.
 
-    Global Instance first_char_premethods : @parser_computational_dataT' _ _ data'
-      := { split_string_for_production str0 valid := first_char_split;
-           split_string_for_production_correct str0 valid it its str := first_char_split_correct_seq (fallback_split_correct_eq it its str) }.
+    Global Instance only_one_nt_premethods : @parser_computational_dataT' _ _ data'
+      := { split_string_for_production str0 valid := only_one_nt_split;
+           split_string_for_production_correct str0 valid it its str := only_one_nt_split_correct_seq }.
 
-    Global Instance first_char_data : @boolean_parser_dataT _ _
+    Global Instance only_one_nt_data : @boolean_parser_dataT _ _
       := { predata := @rdp_list_predata _ G;
            split_stateT := split_stateT;
-           split_string_for_production := first_char_split;
-           split_string_for_production_correct it its str := first_char_split_correct_seq (fallback_split_correct_eq it its str) }.
+           split_string_for_production := only_one_nt_split;
+           split_string_for_production_correct it its str := only_one_nt_split_correct_seq }.
 
     Context (fallback_valid_prod : production CharType -> bool).
 
-    Fixpoint first_char_valid_prod
-             (first_char_valid : string -> bool)
+    Fixpoint only_one_nt_valid_prod
+             (only_one_nt_valid : string -> bool)
              (p : production CharType)
     : bool
       := match p with
            | nil => true
-           | (Terminal _)::p' => first_char_valid_prod first_char_valid p'
-           | (NonTerminal nt)::p' => ((first_char_valid_prod first_char_valid p')
-                                        && first_char_valid nt
+           | (Terminal _)::p' => only_one_nt_valid_prod only_one_nt_valid p'
+           | (NonTerminal nt)::p' => ((only_one_nt_valid_prod only_one_nt_valid p')
+                                        && only_one_nt_valid nt
                                         && (has_only_terminals p' || fallback_valid_prod p))%bool
          end.
 
-    Definition first_char_valid : bool
-      := split_valid (G := G) first_char_valid_prod.
+    Definition only_one_nt_valid : bool
+      := split_valid (G := G) only_one_nt_valid_prod.
 
-    Lemma first_char_valid_prod_cons {fcv x xs}
-    : first_char_valid_prod fcv (x::xs)
+    Lemma only_one_nt_valid_prod_cons {fcv x xs}
+    : only_one_nt_valid_prod fcv (x::xs)
       = match x with
-          | Terminal _ => first_char_valid_prod fcv xs
-          | NonTerminal nt => ((first_char_valid_prod fcv xs)
+          | Terminal _ => only_one_nt_valid_prod fcv xs
+          | NonTerminal nt => ((only_one_nt_valid_prod fcv xs)
                                  && fcv nt
                                  && (has_only_terminals xs || fallback_valid_prod (x::xs)))%bool
         end.
@@ -213,7 +220,7 @@ About RightId.
 
     Lemma valid_if_has_only_terminals {fcv p}
           (H : has_only_terminals p = true)
-    : first_char_valid_prod fcv p = true.
+    : only_one_nt_valid_prod fcv p = true.
     Proof.
       induction p; t_equality.
     Qed.
@@ -221,24 +228,40 @@ About RightId.
     Lemma has_only_terminals_min_parse_length
           {str0 valid strs its}
           (H : has_only_terminals its = true)
-          (p : minimal_parse_of_production String G initial_nonterminal_data
-
- has_only_terminals its = true
-  strs : String
-  X2 : minimal_parse_of_production String G (Valid_nonterminals G)
-         rdp_list_is_valid_nonterminal rdp_list_remove_nonterminal str0 valid
-         strs its
-  H8 : [[c]] ++ strs ≤s str0
-  pf : s1 ++ [[c]] ++ strs ≤s str0
-  st : split_stateT (s1 ++ [[c]] ++ strs)
-  ============================
-   SplitAtT (Length (s1 ++ [[c]] ++ strs) - S (Datatypes.length its))
+          (p : minimal_parse_of_production (String := String) (G := G) str0 valid strs its)
+    : List.length its = Length strs.
+    Proof.
+      generalize dependent strs.
+      induction its; simpl in *.
+      { intros strs p.
+        inversion p; subst.
+        rewrite Length_Empty; reflexivity. }
+      { destruct_head item.
+        { intros strs p.
+          inversion p; subst.
+          inversion_head @minimal_parse_of_item.
+          rewrite <- Length_correct, Singleton_Length, <- IHits by assumption.
+          reflexivity. }
+        { exfalso; discriminate. } }
+    Qed.
 
     Context (fallback_split_ind : forall x xs, fallback_valid_prod (x::xs) -> fallback_valid_prod xs).
+    Context (fallback_split_prod_each
+             : forall nt_it its str0 valid s1 s2 (pf : s1 ++ s2 ≤s str0) st,
+                 has_only_terminals its = false
+                 -> MinimalParse.minimal_parse_of_item (G := G) str0 valid s1 (NonTerminal CharType nt_it)
+                 -> MinimalParse.minimal_parse_of_production (G := G) str0 valid s2 its
+                 -> fallback_valid_prod ((NonTerminal _ nt_it)::its) = true
+                 -> In
+                      (Length s1)
+                      (fallback_split (NonTerminal _ nt_it) its {| string_val := s1 ++ s2; state_val := st |})).
 
-    Lemma first_char_split_complete
-          (H : first_char_valid = true)
-    : forall str0 valid str pf nt,
+    Hint Rewrite NPeano.Nat.add_sub : equality_t_db.
+    Hint Rewrite @has_only_terminals_min_parse_length using eassumption : equality_t_end_db.
+
+    Lemma only_one_nt_split_complete
+          (H : only_one_nt_valid = true)
+    : forall str0 valid (str : StringWithSplitState String split_stateT) (pf : str ≤s str0) nt,
         is_valid_nonterminal initial_nonterminals_data nt ->
         ForallT
           (Forall_tails
@@ -246,11 +269,11 @@ About RightId.
                 match prod with
                   | [] => True
                   | it :: its =>
-                    @split_list_completeT _ String G first_char_data str0 valid str pf
-                                          (@first_char_split it its str) it its
+                    @split_list_completeT _ String G only_one_nt_data str0 valid it its str pf
+                                          (@only_one_nt_split it its str)
                 end)) (Lookup G nt).
     Proof.
-      apply (split_complete_simple first_char_valid_prod).
+      apply (split_complete_simple only_one_nt_valid_prod).
       { intros ? ? ? p.
         induction p; t_equality. }
       { intros f x xs; revert x.
@@ -260,115 +283,26 @@ About RightId.
               In
                 ({| string_val := fst (SplitAt (Length s1) (s1 ++ s2)); state_val := fst st1st2 |},
                  {| string_val := snd (SplitAt (Length s1) (s1 ++ s2)); state_val := snd st1st2 |})
-                (first_char_split it its {| string_val := s1 ++ s2; state_val := st |})}).
+                (only_one_nt_split it its {| string_val := s1 ++ s2; state_val := st |})}).
         { rewrite SplitAt_concat_correct; simpl; trivial. }
         { exists (split_state_at (Length s1) st).
-          unfold first_char_split.
-          t_equality.
-
-          Focus 2.
-          revert st.
-
-          rewrite <- Associativity.
-          {
-unfold SplitAtT; simpl.
-unfold eq_rect.
-            match goal with
-              | [ |- context[match ?e with eq_refl => _ end] ]
-                => subst;
-                  match type of e with
-                    | ?a = ?b
-                      => generalize e;
-                        first [ generalize dependent b; generalize dependent a; intros; progress subst
-                              | generalize dependent a; generalize dependent b; intros; progress subst ]
-                  end
-            end.
-            reflexivity. }
-          { unfold eq_rect; simpl.
-            do 3 match goal with
-                   | [ |- context[match ?e with eq_refl => _ end] ]
-                     => subst;
-                       let T := type of e in
-                       match eval simpl in T with
-                         | ?a = ?b
-                           => generalize e;
-                             first [ generalize dependent b; generalize dependent a; intros; progress subst
-                                   | generalize dependent a; generalize dependent b; intros; progress subst ]
-                       end
-                   | _ => progress simpl
-                 end.
-            reflexivity. }
-          { unfold eq_rect; simpl.
-            match goal with
-                   | [ |- context[match ?e with eq_refl => _ end] ]
-                     => subst;
-                       let T := type of e in
-                       match eval simpl in T with
-                         | ?a = ?b
-                           => generalize e; simpl;
-                             first [ generalize dependent b; intros; progress subst
-                                   | generalize dependent a; generalize dependent b; intros; progress subst
-                                   | generalize b; intros; progress subst
-                                   | generalize a; generalize dependent b; intros; progress subst
-                                   | generalize dependent a; generalize b; intros; progress subst
-                                   | generalize a; generalize b; intros; progress subst ]
-                       end
-                   | _ => progress simpl
-                 end.
-            reflexivity. }
-          {
-unfold SplitAtT; simpl.
-          generalize
-                                                        e
-
-          generalize (RightId String [[ c ]]).
-          general
-
- }
+          unfold only_one_nt_split.
+          t_equality;
+            try solve [ rewrite has_only_terminals_min_parse_length by eassumption;
+                        rewrite NPeano.Nat.add_sub;
+                        reflexivity
+                      | eapply fallback_split_prod_each;
+                        repeat first [ eassumption
+                                     | constructor ] ]. } }
       { exact H. }
     Qed.
 
-    Global Instance first_char_cdata' H : @boolean_parser_completeness_dataT' _ _ G first_char_data
-      := { remove_nonterminal_1 := rdp_list_remove_nonterminal_1;
-           remove_nonterminal_2 := rdp_list_remove_nonterminal_2;
-           split_string_for_production_complete := @first_char_split_complete H }.
+    Global Instance only_one_nt_cdata' H : @boolean_parser_completeness_dataT' _ _ G only_one_nt_data
+      := { split_string_for_production_complete := @only_one_nt_split_complete H }.
 
-    Global Instance first_char_cdata H : @boolean_parser_correctness_dataT _ _ G
-      := { data := first_char_data;
-           cdata' := first_char_cdata' H }.
-  End first_char_splitter.
+    Global Instance only_one_nt_cdata H : @boolean_parser_correctness_dataT _ _ G
+      := { data := only_one_nt_data;
+           rdata' := rdp_list_rdata';
+           cdata' := only_one_nt_cdata' H }.
+  End only_one_nt_splitter.
 End StringT.
-
-Section on_ab_star.
-  Definition ab_star_linear_split := first_char_split (String := string_stringlike) (fun _ _ _ => nil).
-  Definition ab_star_linear_split_correct_seq {it its str} : List.Forall _ _
-    := @first_char_split_correct_seq _ string_stringlike (fun _ _ _ => nil) it its str (Forall_nil _).
-
-  Global Instance ab_star_premethods : @parser_computational_dataT' _ string_stringlike (@rdp_list_data' _ _ ab_star_grammar)
-    := first_char_premethods (fun _ _ _ => nil) ab_star_grammar (fun _ _ _ => Forall_nil _).
-  Global Instance ab_star_data : @boolean_parser_dataT _ string_stringlike
-    := first_char_data (fun _ _ _ => nil) ab_star_grammar (fun _ _ _ => Forall_nil _).
-
-  Global Instance ab_star_cdata' : @boolean_parser_completeness_dataT' _ _ ab_star_grammar ab_star_data
-    := first_char_cdata' (fun _ _ _ => nil) ab_star_grammar (fun _ _ _ => Forall_nil _) eq_refl.
-
-  Global Instance ab_star_cdata : @boolean_parser_correctness_dataT _ _ ab_star_grammar
-    := first_char_cdata (String := string_stringlike) (fun _ _ _ => nil) ab_star_grammar (fun _ _ _ => Forall_nil _) eq_refl.
-End on_ab_star.
-
-Section on_ab_star'.
-  Definition ab_star'_linear_split := first_char_split (String := string_stringlike) (fun _ _ _ => nil).
-  Definition ab_star'_linear_split_correct_seq {it its str} : List.Forall _ _
-    := @first_char_split_correct_seq _ string_stringlike (fun _ _ _ => nil) it its str (Forall_nil _).
-
-  Global Instance ab_star'_premethods : @parser_computational_dataT' _ string_stringlike (@rdp_list_data' _ _ ab_star_grammar')
-    := first_char_premethods (fun _ _ _ => nil) ab_star_grammar' (fun _ _ _ => Forall_nil _).
-  Global Instance ab_star'_data : @boolean_parser_dataT _ string_stringlike
-    := first_char_data (fun _ _ _ => nil) ab_star_grammar' (fun _ _ _ => Forall_nil _).
-
-  Global Instance ab_star'_cdata' : @boolean_parser_completeness_dataT' _ _ ab_star_grammar' ab_star'_data
-    := first_char_cdata' (fun _ _ _ => nil) ab_star_grammar' (fun _ _ _ => Forall_nil _) eq_refl.
-
-  Global Instance ab_star'_cdata : @boolean_parser_correctness_dataT _ _ ab_star_grammar'
-    := first_char_cdata (String := string_stringlike) (fun _ _ _ => nil) ab_star_grammar' (fun _ _ _ => Forall_nil _) eq_refl.
-End on_ab_star'.
